Cleanup

src/Util.v
@@ -2,41 +2,44 @@ Require Import Coq.Lists.List.
 Import ListNotations.
 Require Import Coq.micromega.Lia.
 
-Fixpoint iter' {A: Type} (m n: nat) (f: nat -> A -> A) (a: A) : A :=
+Create HintDb iter discriminated.
+
+Fixpoint iter' (A: Type) (m n: nat) (f: nat -> A -> A) (a: A) : A :=
   match m with
   | O => a
-  | S m' => iter' m' n f (f (n-m) a)
+  | S m' => iter' A m' n f (f (n-m) a)
   end.
-
-Definition iter {A: Type} (n: nat) := @iter' A n n.
-
-
-Hint Unfold iter.
-
-Lemma iter'_S {A: Type}:
-  forall f i j (a: A),
-    iter' (S i) (S j) f a = f j (iter' i j f a).
+  
+Lemma iter'_S:
+  forall A f i j (a: A),
+  iter' A (S i) (S j) f a = f j (iter' A i j f a).
 Proof.
   induction i; intros.
   - simpl. replace (j - 0) with j by lia. reflexivity.
-  - simpl. apply IHi.
+  - eauto.
 Qed.
 
+Local Hint Rewrite iter'_S : iter.
+Definition iter (A: Type) (n: nat) := @iter' A n n.
+Local Hint Unfold iter : iter.
+
 Theorem iter_inv {A: Type}:
-  forall (P: nat -> A -> Prop) f a,
-  P 0 a ->
-  (forall j b, P j b -> P (S j) (f j b)) ->
-  (forall i, P i (iter i f a)).
+  forall (Inv: nat -> A -> Prop) f a,
+  Inv 0 a ->
+  (forall j b, Inv j b -> Inv (S j) (f j b)) ->
+  (forall i, Inv i (iter A i f a)).
 Proof.
-  intros. induction i; intros.
-  - auto.
-  - apply H0 in IHi.
-    replace (iter (S i) f a) with (f i (iter i f a)); auto.
+  induction i; intros; eauto.
+  - replace (iter A (S i) f a) with (f i (iter A i f a)); auto.
     unfold iter. rewrite iter'_S. reflexivity.
 Qed.
 
+Arguments iter {A}.
+
 
 (* Section _iter.
+Print iter.
+Definition xs := [0;1;2;3].
 Definition arith_sum := iter (length xs) (fun i x => x + nth i xs 0) 0.
 Compute arith_sum.
 Theorem arith_sum_correct:
