src/circomlib/bitify.v
@@ -31,38 +31,25 @@ Local Infix "-" := sub. Local Infix "/" := div.
 Require Import Coq.Lists.List.
 Local Open Scope list_scope.
 
-Theorem fold_right_invariant
-  (A B: Type)
-  (l: list B)
-  (f: B -> A -> A)
-  (a0: A) 
-  (P: list B -> A -> Prop)
-  (Hinit: P nil a0)
-  (Hinv: forall a b bs, P bs a -> P (b::bs) (f b a)):
-  P l (fold_right f a0 l).
-Proof.
-  induction l; eauto.
-Qed.
-
-Definition uncurry {X Y Z : Type}
-  (f : X -> Y -> Z) (p : X * Y) : Z.
-Proof. destruct p; apply f; eauto. Defined.
-
-Local Open Scope nat_scope.
-Definition fold_i {A B: Type} (f: nat -> B -> A -> A) (a0: A) :=
-  fold_right (fun b (ia: (nat * A)) => let (i,a):= ia in (i+1, f i b a)) (0,a0).
-Local Close Scope nat_scope.
 Require Import Coq.PArith.BinPosDef.
-
+Require Import Util.
+Require Import Coq.Arith.PeanoNat.
+From Coq Require Import Lia.
+Require Import Coq.Arith.Compare_dec.
+Require Import Crypto.Util.Decidable.
+(* Require Import Crypto.Arithmetic.PrimeFieldTheorems. *)
 
 (* Context (m:positive) {prime_m:prime m}. *)
 
-Require Import Util.
+Definition binary (x: F) := x = zero \/ x = one.
+
+Definition sum (xs: list F) := fold_right add zero xs.
 
 Definition Num2Bits n (_in: F) (_out: tuple (F) n) : Prop :=
   let lc1 := zero in
   let e2 := one in
-  match (iter n (fun i acc =>
+  match (iter n
+    (fun i acc =>
       match acc with
       | (lc1, e2, _C) =>
         let out_i := (Tuple.nth_default zero i _out) in
@@ -74,14 +61,6 @@ Definition Num2Bits n (_in: F) (_out: tuple (F) n) : Prop :=
   | (lc1, e2, _C) => (lc1 = _in) /\ _C
   end.
 
-Definition binary (x: F) := x = zero \/ x = one.
-
-Definition sum (xs: list F) := fold_right add zero xs.
-
-Require Import Coq.Arith.PeanoNat.
-
-(* Definition bits2num (_out: list (F)) := fold_right (fun (F.pow 2) *)
-
 Definition Num2Bits_spec n (_in: F) (_out: tuple F n) :=
   (forall i, Nat.lt i n -> binary (Tuple.nth_default zero i _out)).
 
@@ -90,62 +69,52 @@ Definition Num2Bits_inv n (_out: tuple F n) i (acc: (F * F * Prop)) :=
   | (lc1, e2, _C) =>
     _C -> forall j, Nat.lt j i -> binary (Tuple.nth_default zero j _out)
   end.
-  
-(* Compute (Num2Bits_inv 5 0). *)
-
-From Coq Require Import Lia.
-Require Import Coq.Arith.Compare_dec.
-Require Import Crypto.Util.Decidable.
-
-Require Import Crypto.Arithmetic.PrimeFieldTheorems.
 
 Theorem Num2Bits_correct n _in _out:
   Num2Bits n _in _out -> Num2Bits_spec n _in _out.
 Proof using Type*.
   unfold Num2Bits, Num2Bits_spec.
-  intros.
-  pose proof (@iter_inv _ (Num2Bits_inv n _out)).
-  remember (fun (i : nat) (acc : bitify.F * bitify.F * Prop) =>
-  let (y, _C) := acc in
-  let (lc1, e2) := y in
-  (lc1 + Tuple.nth_default 0 i _out * e2, e2 + e2,
-  Tuple.nth_default 0 i _out * (Tuple.nth_default 0 i _out - 1) = 0 /\
-  _C)) as f.
+  intros prog i H_i_lt_n.
+  pose proof (iter_inv (Num2Bits_inv n _out)) as Hinv.
+  (* iter initialization *)
   remember (0, 1, True) as a0.
-  assert (Num2Bits_inv n _out 0 a0).
+  (* iter function *)
+  remember (fun (i : nat) (acc : bitify.F * bitify.F * Prop) =>
+    let (y, _C) := acc in
+    let (lc1, e2) := y in
+    (lc1 + Tuple.nth_default 0 i _out * e2, e2 + e2,
+    Tuple.nth_default 0 i _out * (Tuple.nth_default 0 i _out - 1) = 0 /\
+    _C)) as f.
+  (* Prove Inv hold for initialization *)
+  assert (Hinit: Num2Bits_inv n _out 0 a0).
   {
     unfold Num2Bits_inv.
-    rewrite Heqa0. intuition.
+    rewrite Heqa0. intros _ j H_j_lt_0.
     unfold binary. left. lia.
   }
-  specialize (H1 f a0).
-  specialize (H1 H2).
-  assert (forall (j : nat) (b : bitify.F * bitify.F * Prop),
-  Num2Bits_inv n _out j b -> Num2Bits_inv n _out (S j) (f j b)).
+  (* Prove Inv is inductive *)
+  assert (Hind: forall (j : nat) (b : bitify.F * bitify.F * Prop),
+    Num2Bits_inv n _out j b -> Num2Bits_inv n _out (S j) (f j b)).
   {
     unfold Num2Bits_inv.
-    intros.
-    destruct b. destruct p.
+    intros j res Hprev.
+    destruct res. destruct p.
     rewrite Heqf.
-    intros.
-    destruct H4.
-    specialize (H3 H6).
-    assert (Nat.le j0 j). lia.
+    intros Hstep j0 H_j0_lt.
+    destruct Hstep as [Hstep HP].
+    specialize  (Hprev HP).
+    assert (H_j0_leq: Nat.le j0 j) by lia.
     destruct (lt_dec j0 j).
-    - apply H3. trivial.
-    - assert (Nat.eq j0 j) by lia. unfold binary. {
-      destruct (dec (Tuple.nth_default 0 j0 _out = 0)).
-      + left. trivial.
-      + right. rewrite H8 in *. Field.fsatz.
-    }
+    - auto.
+    - unfold binary.
+      replace j0 with j by lia.
+      destruct (dec (Tuple.nth_default 0 j _out = 0)).
+      + auto.
+      + right. Field.fsatz.
   }
-  specialize (H1 H3).
-  unfold Num2Bits_inv in H1.
-  specialize (H1 n).
+  specialize (Hinv f a0 Hinit Hind n).
+  unfold Num2Bits_inv in Hinv.
   destruct (iter n f a0).
   destruct p.
-  destruct H.
-  specialize (H1 H4).
-  apply H1.
-  lia.
+  intuition.
 Qed.
